Simplify stack programs

theories/logrel/F_mu_ref_conc/examples/lock.v
@@ -7,20 +7,26 @@ Definition newlock : expr := Alloc (#♭ false).
 Definition acquire : expr :=
   Rec (If (CAS (Var 1) (#♭ false) (#♭ true)) (Unit) (App (Var 0) (Var 1))).
 (** [release = λ x. x <- false] *)
-Definition release : expr := Rec (Store (Var 1) (#♭ false)).
+Definition release : expr := Lam (Store (Var 0) (#♭ false)).
 (** [with_lock e l = λ x. (acquire l) ;; e x ;; (release l)] *)
 Definition with_lock (e : expr) (l : expr) : expr :=
-  Rec
-    (App (Rec (App (Rec (App (Rec (Var 3)) (App release l.[ren (+6)])))
-                   (App e.[ren (+4)] (Var 3))))
-         (App acquire l.[ren (+2)])
+  Lam
+    (Seq
+       (App acquire l.[ren (+1)])
+       (LetIn
+          (App e.[ren (+1)] (Var 0))
+          (Seq (App release l.[ren (+2)]) (Var 0))
+       )
     ).
 
 Definition with_lockV (e l : expr) : val :=
-  RecV
-    (App (Rec (App (Rec (App (Rec (Var 3)) (App release l.[ren (+6)])))
-                   (App e.[ren (+4)] (Var 3))))
-         (App acquire l.[ren (+2)])
+  LamV
+    (Seq
+       (App acquire l.[ren (+1)])
+       (LetIn
+          (App e.[ren (+1)] (Var 0))
+          (Seq (App release l.[ren (+2)]) (Var 0))
+       )
     ).
 
 Lemma with_lock_to_val e l : to_val (with_lock e l) = Some (with_lockV e l).
@@ -29,6 +35,7 @@ Proof. trivial. Qed.
 Lemma with_lock_of_val e l : of_val (with_lockV e l) = with_lock e l.
 Proof. trivial. Qed.
 
+Global Typeclasses Opaque with_lockV.
 Global Opaque with_lockV.
 
 Lemma newlock_closed f : newlock.[f] = newlock.
@@ -43,14 +50,9 @@ Lemma release_closed f : release.[f] = release.
 Proof. by asimpl. Qed.
 Hint Rewrite release_closed : autosubst.
 
-Lemma with_lock_subst (e l : expr) f :  (with_lock e l).[f] = with_lock e.[f] l.[f].
+Lemma with_lock_subst (e l : expr) f :
+  (with_lock e l).[f] = with_lock e.[f] l.[f].
 Proof. unfold with_lock; asimpl; trivial. Qed.
-
-Lemma with_lock_closed e l:
-  (∀ f : var → expr, e.[f] = e) →
-  (∀ f : var → expr, l.[f] = l) →
-  ∀ f, (with_lock e l).[f] = with_lock e l.
-Proof. asimpl => H1 H2 f. unfold with_lock. by rewrite ?H1 ?H2. Qed.
 
 Definition LockType := Tref TBool.
 
@@ -68,18 +70,20 @@ Lemma with_lock_type e l Γ τ τ' :
   typed Γ l LockType →
   typed Γ (with_lock e l) (TArrow τ τ').
 Proof.
-  intros H1 H2. do 3 econstructor; eauto.
-  - repeat (econstructor; eauto using release_type).
-    + eapply (context_weakening [_; _; _; _; _; _]); eauto.
-    + eapply (context_weakening [_; _; _; _]); eauto.
-  - eapply acquire_type.
-  - eapply (context_weakening [_; _]); eauto.
+  intros ??.
+  do 3 econstructor; eauto using acquire_type.
+  - eapply (context_weakening [_]); eauto.
+  - econstructor; eauto using typed.
+    eapply (context_weakening [_]); eauto.
+  - econstructor; eauto using typed.
+    econstructor; eauto using release_type.
+    eapply (context_weakening [_;_]); eauto.
 Qed.
 
 Section proof.
   Context `{cfgSG Σ}.
   Context `{heapIG Σ}.
-  
+
   Lemma steps_newlock E ρ j K :
     nclose specN ⊆ E →
     spec_ctx ρ ∗ j ⤇ fill K newlock
@@ -89,6 +93,7 @@ Section proof.
     by iMod (step_alloc _ _ j K with "[Hj]") as "Hj"; eauto.
   Qed.
 
+  Global Typeclasses Opaque newlock.
   Global Opaque newlock.
 
   Lemma steps_acquire E ρ j K l :
@@ -107,6 +112,7 @@ Section proof.
     Unshelve. all:trivial.
   Qed.
 
+  Global Typeclasses Opaque acquire.
   Global Opaque acquire.
 
   Lemma steps_release E ρ j K l b:
@@ -115,48 +121,45 @@ Section proof.
       ⊢ |={E}=> j ⤇ fill K Unit ∗ l ↦ₛ (#♭v false).
   Proof.
     iIntros (HNE) "[#Hspec [Hl Hj]]". unfold release.
-    iMod (step_rec _ _ j K with "[Hj]") as "Hj"; eauto; try done.
-    iMod (step_store _ _ j K _ _ _ _ _ with "[Hj Hl]") as "[Hj Hl]"; eauto.
-    { by iFrame. }
+    iMod (do_step_pure with "[$Hj]") as "Hj"; eauto; try done.
+    iMod (step_store with "[$Hj $Hl]") as "[Hj Hl]"; eauto.
     by iIntros "!> {$Hj $Hl}".
-    Unshelve. all: trivial.
   Qed.
 
+  Global Typeclasses Opaque release.
   Global Opaque release.
 
   Lemma steps_with_lock E ρ j K e l P Q v w:
     nclose specN ⊆ E →
-    (∀ f, e.[f] = e) (* e is a closed term *) →
+    (* (∀ f, e.[f] = e) (* e is a closed term *) → *)
     (∀ K', spec_ctx ρ ∗ P ∗ j ⤇ fill K' (App e (of_val w))
             ⊢ |={E}=> j ⤇ fill K' (of_val v) ∗ Q) →
     spec_ctx ρ ∗ P ∗ l ↦ₛ (#♭v false)
                 ∗ j ⤇ fill K (App (with_lock e (Loc l)) (of_val w))
       ⊢ |={E}=> j ⤇ fill K (of_val v) ∗ Q ∗ l ↦ₛ (#♭v false).
   Proof.
-    iIntros (HNE H1 H2) "[#Hspec [HP [Hl Hj]]]".
-    iMod (step_rec _ _ j K _ _ _ _ with "[Hj]") as "Hj"; eauto.
-    iAsimpl. rewrite H1.
-    iMod (steps_acquire _ _ j ((AppRCtx (RecV _)) :: K)
-                   _ _ with "[Hj Hl]") as "[Hj Hl]"; eauto.
-    { simpl. iFrame "Hspec Hj Hl"; eauto. }
-    simpl.
-    iMod (step_rec _ _ j K _ _ _ _ with "[Hj]") as "Hj"; eauto.
-    iAsimpl. rewrite H1.
-    iMod (H2 ((AppRCtx (RecV _)) :: K) with "[Hj HP]") as "[Hj HQ]"; eauto.
-    { simpl. iFrame "Hspec Hj HP"; eauto. }
-    simpl.
-    iMod (step_rec _ _ j K _ _ _ _ with "[Hj]") as "Hj"; eauto.
+    iIntros (HNE He) "[#Hspec [HP [Hl Hj]]]".
+    iMod (do_step_pure with "[$Hj]") as "Hj"; eauto.
     iAsimpl.
-    iMod (steps_release _ _ j ((AppRCtx (RecV _)) :: K) _ _ with "[Hj Hl]")
+    iMod (steps_acquire _ _ j (SeqCtx _ :: K) with "[$Hj Hl]") as "[Hj Hl]";
+      auto. simpl.
+    iMod (do_step_pure with "[$Hj]") as "Hj"; eauto.
+    iMod (He (LetInCtx _ :: K) with "[$Hj HP]") as "[Hj HQ]"; eauto.
+    simpl.
+    iMod (do_step_pure with "[$Hj]") as "Hj"; eauto.
+    iAsimpl.
+    iMod (steps_release _ _ j (SeqCtx _ :: K) _ _ with "[$Hj $Hl]")
       as "[Hj Hl]"; eauto.
-    { simpl. by iFrame. }
-    rewrite ?fill_app /=.
-    iMod (step_rec _ _ j K _ _ _ _ with "[Hj]") as "Hj"; eauto.
-    iAsimpl. iModIntro; by iFrame.
-    Unshelve.
-    all: try match goal with |- to_val _ = _ => auto using to_of_val end.
-    trivial.
+    simpl.
+    iMod (do_step_pure with "[$Hj]") as "Hj"; eauto.
+    iModIntro; by iFrame.
   Qed.
 
+  Global Typeclasses Opaque with_lock.
   Global Opaque with_lock.
 End proof.
+
+Global Hint Rewrite newlock_closed : autosubst.
+Global Hint Rewrite acquire_closed : autosubst.
+Global Hint Rewrite release_closed : autosubst.
+Global Hint Rewrite with_lock_subst : autosubst.
