theories/logrel/F_mu_ref_conc/examples/stack/CG_stack.v
@@ -7,33 +7,34 @@ Definition CG_StackType τ :=
 
 (* Coarse-grained push *)
 Definition CG_push (st : expr) : expr :=
-  Rec (Store
-         (st.[ren (+2)]) (Fold (InjR (Pair (Var 1) (Load st.[ren (+ 2)]))))).
+  Lam (Store (st.[ren (+1)]) (Fold (InjR (Pair (Var 0) (Load st.[ren (+ 1)]))))).
 
 Definition CG_locked_push (st l : expr) := with_lock (CG_push st) l.
 Definition CG_locked_pushV (st l : expr) : val := with_lockV (CG_push st) l.
 
 Definition CG_pop (st : expr) : expr :=
-  Rec (Case (Unfold (Load st.[ren (+ 2)]))
+  Lam (Case (Unfold (Load st.[ren (+ 1)]))
             (InjL Unit)
             (
-              App (Rec (InjR (Fst (Var 2))))
-                  (Store st.[ren (+ 3)] (Snd (Var 0)))
+              Seq
+                (Store st.[ren (+ 2)] (Snd (Var 0)))
+                (InjR (Fst (Var 0)))
             )
       ).
 
 Definition CG_locked_pop (st l : expr) := with_lock (CG_pop st) l.
 Definition CG_locked_popV (st l : expr) : val := with_lockV (CG_pop st) l.
 
-Definition CG_snap (st l : expr) :=  with_lock (Rec (Load st.[ren (+2)])) l.
-Definition CG_snapV (st l : expr) : val := with_lockV (Rec (Load st.[ren (+2)])) l.
+Definition CG_snap (st l : expr) :=  with_lock (Lam (Load st.[ren (+1)])) l.
+Definition CG_snapV (st l : expr) : val := with_lockV (Lam (Load st.[ren (+1)])) l.
 
 Definition CG_iter (f : expr) : expr :=
   Rec (Case (Unfold (Var 1))
             Unit
             (
-              App (Rec (App (Var 3) (Snd (Var 2))))
-                  (App f.[ren (+3)] (Fst (Var 0)))
+              Seq
+                (App f.[ren (+3)] (Fst (Var 0)))
+                (App (Var 1) (Snd (Var 0)))
             )
       ).
 
@@ -41,20 +42,26 @@ Definition CG_iterV (f : expr) : val :=
   RecV (Case (Unfold (Var 1))
             Unit
             (
-              App (Rec (App (Var 3) (Snd (Var 2))))
-                  (App f.[ren (+3)] (Fst (Var 0)))
+              Seq
+                (App f.[ren (+3)] (Fst (Var 0)))
+                (App (Var 1) (Snd (Var 0)))
             )
       ).
 
 Definition CG_snap_iter (st l : expr) : expr :=
-  Rec (App (CG_iter (Var 1)) (App (CG_snap st.[ren (+2)] l.[ren (+2)]) Unit)).
+  Lam (App (CG_iter (Var 0)) (App (CG_snap st.[ren (+1)] l.[ren (+1)]) Unit)).
+
 Definition CG_stack_body (st l : expr) : expr :=
   Pair (Pair (CG_locked_push st l) (CG_locked_pop st l))
        (CG_snap_iter st l).
 
 Definition CG_stack : expr :=
-  TLam (App (Rec (App (Rec (CG_stack_body (Var 1) (Var 3)))
-                (Alloc (Fold (InjL Unit))))) newlock).
+  TLam (
+      LetIn
+        newlock
+        (LetIn
+           (Alloc (Fold (InjL Unit)))
+           (CG_stack_body (Var 0) (Var 1)))).
 
 Section CG_Stack.
   Context `{heapIG Σ, cfgSG Σ}.
@@ -64,17 +71,15 @@ Section CG_Stack.
     typed Γ (CG_push st) (TArrow τ TUnit).
   Proof.
     intros H1. repeat econstructor.
-    eapply (context_weakening [_; _]); eauto.
+    eapply (context_weakening [_]); eauto.
     repeat constructor; asimpl; trivial.
-    eapply (context_weakening [_; _]); eauto.
+    eapply (context_weakening [_]); eauto.
   Qed.
-
-  Lemma CG_push_closed (st : expr) :
-    (∀ f, st.[f] = st) → ∀ f, (CG_push st).[f] = CG_push st.
-  Proof. intros Hst f. unfold CG_push. asimpl. rewrite ?Hst; trivial. Qed.
 
   Lemma CG_push_subst (st : expr) f : (CG_push st).[f] = CG_push st.[f].
   Proof. unfold CG_push; asimpl; trivial. Qed.
+
+  Global Hint Rewrite CG_push_subst : autosubst.
 
   Lemma steps_CG_push E ρ j K st v w :
     nclose specN ⊆ E →
@@ -82,19 +87,17 @@ Section CG_Stack.
     ⊢ |={E}=> j ⤇ fill K Unit ∗ st ↦ₛ FoldV (InjRV (PairV w v)).
   Proof.
     intros HNE. iIntros "[#Hspec [Hx Hj]]". unfold CG_push.
-    iMod (step_rec _ _ j K _ _ _ _ with "[Hj]") as "Hj"; eauto.
+    iMod (do_step_pure with "[$Hj]") as "Hj"; eauto.
     iAsimpl.
     iMod (step_load _ _ j (PairRCtx _ :: InjRCtx :: FoldCtx :: StoreRCtx (LocV _) :: K)
-                    _ _ _ with "[Hj Hx]") as "[Hj Hx]"; eauto.
-    simpl. iFrame "Hspec Hj"; trivial. simpl.
-    iMod (step_store _ _ j K _ _ _ _ _ with "[Hj Hx]") as "[Hj Hx]"; eauto.
-    { by iFrame. }
+            with "[$Hj $Hx]") as "[Hj Hx]"; eauto.
+    simpl.
+    iMod (step_store _ _ j K with "[$Hj $Hx]") as "[Hj Hx]"; eauto.
+    { rewrite /= !to_of_val //. }
     iModIntro. by iFrame.
-    Unshelve.
-    all: try match goal with |- to_val _ = _ => auto using to_of_val end.
-    simpl; by rewrite ?to_of_val.
   Qed.
 
+  Global Typeclasses Opaque CG_push.
   Global Opaque CG_push.
 
   Lemma CG_locked_push_to_val st l :
@@ -106,7 +109,6 @@ Section CG_Stack.
   Proof. trivial. Qed.
 
   Global Opaque CG_locked_pushV.
-
   Lemma CG_locked_push_type st l Γ τ :
     typed Γ st (Tref (CG_StackType τ)) →
     typed Γ l LockType →
@@ -116,17 +118,11 @@ Section CG_Stack.
     eapply with_lock_type; auto using CG_push_type.
   Qed.
 
-  Lemma CG_locked_push_closed (st l : expr) :
-    (∀ f, st.[f] = st) → (∀ f, l.[f] = l) →
-    ∀ f, (CG_locked_push st l).[f] = CG_locked_push st l.
-  Proof.
-    intros H1 H2 f. asimpl. unfold CG_locked_push.
-    rewrite with_lock_closed; trivial. apply CG_push_closed; trivial.
-  Qed.
-
   Lemma CG_locked_push_subst (st l : expr) f :
     (CG_locked_push st l).[f] = CG_locked_push st.[f] l.[f].
-  Proof. by rewrite with_lock_subst CG_push_subst. Qed.
+  Proof. by rewrite /CG_locked_push; asimpl. Qed.
+
+  Hint Rewrite CG_locked_push_subst : autosubst.
 
   Lemma steps_CG_locked_push E ρ j K st w v l :
     nclose specN ⊆ E →
@@ -135,14 +131,13 @@ Section CG_Stack.
     ⊢ |={E}=> j ⤇ fill K Unit ∗ st ↦ₛ FoldV (InjRV (PairV w v)) ∗ l ↦ₛ (#♭v false).
   Proof.
     intros HNE. iIntros "[#Hspec [Hx [Hl Hj]]]". unfold CG_locked_push.
-    iMod (steps_with_lock
-            _ _ j K _ _ _ _ UnitV _ _ _ with "[Hj Hx Hl]") as "Hj"; last done.
-    - iIntros (K') "[#Hspec Hxj]".
-      iApply steps_CG_push; first done. iFrame. trivial.
-    - iFrame "Hspec Hj Hx"; trivial.
-      Unshelve. all: trivial.
+    iMod (steps_with_lock _ _ _ _ _ _ (st ↦ₛ v)%I _ UnitV with "[$Hj $Hx $Hl]")
+      as "Hj"; auto.
+    iIntros (K') "[#Hspec Hxj]".
+    iApply steps_CG_push; first done. by iFrame.
   Qed.
 
+  Global Typeclasses Opaque CG_locked_push.
   Global Opaque CG_locked_push.
 
   (* Coarse-grained pop *)
@@ -152,22 +147,22 @@ Section CG_Stack.
   Proof.
     intros H1.
     econstructor.
-    eapply (Case_typed _ _ _ _ TUnit);
-      [| repeat constructor
-       | repeat econstructor; eapply (context_weakening [_; _; _]); eauto].
-    replace (TSum TUnit (TProd τ (CG_StackType τ))) with
-    ((TSum TUnit (TProd τ.[ren (+1)] (TVar 0))).[(CG_StackType τ)/])
-      by (by asimpl).
-    repeat econstructor.
-    eapply (context_weakening [_; _]); eauto.
+    eapply (Case_typed _ _ _ _ TUnit); eauto using typed.
+    - replace (TSum TUnit (TProd τ (CG_StackType τ))) with
+          ((TSum TUnit (TProd τ.[ren (+1)] (TVar 0))).[(CG_StackType τ)/])
+        by (by asimpl).
+      repeat econstructor.
+      eapply (context_weakening [_]); eauto.
+    - econstructor; eauto using typed.
+      econstructor; eauto using typed.
+      eapply (context_weakening [_; _]); eauto.
   Qed.
 
-  Lemma CG_pop_closed (st : expr) :
-    (∀ f, st.[f] = st) → ∀ f, (CG_pop st).[f] = CG_pop st.
-  Proof. intros Hst f. unfold CG_pop. asimpl. rewrite ?Hst; trivial. Qed.
+  Lemma CG_pop_subst (st : expr) f :
+    (CG_pop st).[f] = CG_pop st.[f].
+  Proof. by rewrite /CG_pop; asimpl. Qed.
 
-  Lemma CG_pop_subst (st : expr) f : (CG_pop st).[f] = CG_pop st.[f].
-  Proof. unfold CG_pop; asimpl; trivial. Qed.
+  Hint Rewrite CG_pop_subst : autosubst.
 
   Lemma steps_CG_pop_suc E ρ j K st v w :
     nclose specN ⊆ E →
@@ -176,35 +171,25 @@ Section CG_Stack.
       ⊢ |={E}=> j ⤇ fill K (InjR (of_val w)) ∗ st ↦ₛ v.
   Proof.
     intros HNE. iIntros "[#Hspec [Hx Hj]]". unfold CG_pop.
-    iMod (step_rec _ _ j K _ _ _ _ with "[Hj]") as "Hj"; eauto.
+    iMod (do_step_pure with "[$Hj]") as "Hj"; eauto.
     iAsimpl.
-    iMod (step_load _ _ j (UnfoldCtx :: CaseCtx _ _ :: K)
-                    _ _ _ with "[Hj Hx]") as "[Hj Hx]"; eauto.
-    rewrite ?fill_app. simpl.
-    iFrame "Hspec Hj"; trivial.
-    rewrite ?fill_app. simpl.
-    iMod (step_Fold  _ _ j (CaseCtx _ _ :: K)
-                    _ _ _ _ with "[Hj]") as "Hj"; eauto.
+    iMod (step_load _ _ _ (UnfoldCtx :: CaseCtx _ _ :: K)  with "[$Hj $Hx]")
+      as "[Hj Hx]"; eauto.
     simpl.
-    iMod (step_case_inr _ _ j K _ _ _ _ _ with "[Hj]") as "Hj"; eauto.
+    iMod (do_step_pure  _ _ _ (CaseCtx _ _ :: K) with "[$Hj]") as "Hj"; eauto.
+    simpl.
+    iMod (do_step_pure with "[$Hj]") as "Hj"; eauto.
     iAsimpl.
-    iMod (step_snd _ _ j (StoreRCtx (LocV _) :: AppRCtx (RecV _) :: K) _ _ _ _
-                   _ _ with "[Hj]") as "Hj"; eauto.
+    iMod (do_step_pure _ _ _ (StoreRCtx (LocV _) :: SeqCtx _ :: K)
+            with "[$Hj]") as "Hj"; eauto.
     simpl.
-    iMod (step_store _ _ j (AppRCtx (RecV _) :: K) _ _ _ _ _ _
-          with "[Hj Hx]") as "[Hj Hx]"; eauto.
-    rewrite ?fill_app. simpl.
-    iFrame "Hspec Hj"; trivial.
-    rewrite ?fill_app. simpl.
-    iMod (step_rec _ _ j K _ _ _ _ with "[Hj]") as "Hj"; eauto.
-    iAsimpl.
-    iMod (step_fst _ _ j (InjRCtx :: K) _ _ _ _ _ _
-          with "[Hj]") as "Hj"; eauto.
+    iMod (step_store _ _ j (SeqCtx _ :: K) with "[$Hj $Hx]") as "[Hj Hx]";
+      eauto using to_of_val.
     simpl.
-    iModIntro. iFrame "Hj Hx"; trivial.
-    Unshelve.
-    all: try match goal with |- to_val _ = _ => simpl; by rewrite ?to_of_val end.
-    all: trivial.
+    iMod (do_step_pure with "[$Hj]") as "Hj"; eauto.
+    iMod (do_step_pure _ _ _ (InjRCtx :: K) with "[$Hj]") as "Hj"; eauto.
+    simpl.
+    by iFrame "Hj Hx".
   Qed.
 
   Lemma steps_CG_pop_fail E ρ j K st :
@@ -214,21 +199,17 @@ Section CG_Stack.
       ⊢ |={E}=> j ⤇ fill K (InjL Unit) ∗ st ↦ₛ FoldV (InjLV UnitV).
   Proof.
     iIntros (HNE) "[#Hspec [Hx Hj]]". unfold CG_pop.
-    iMod (step_rec _ _ j K _ _ _ _ with "[Hj]") as "Hj"; eauto.
+    iMod (do_step_pure with "[$Hj]") as "Hj"; eauto.
     iAsimpl.
     iMod (step_load _ _ j (UnfoldCtx :: CaseCtx _ _ :: K)
-                    _ _ _ with "[Hj Hx]") as "[Hj Hx]"; eauto.
-    simpl. iFrame "Hspec Hj"; trivial. simpl.
-    iMod (step_Fold _ _ j (CaseCtx _ _ :: K)
-                    _ _ _ _ with "[Hj]") as "Hj"; eauto.
-    iMod (step_case_inl _ _ j K _ _ _ _ _ with "[Hj]") as "Hj"; eauto.
-    iAsimpl.
-    iModIntro. iFrame "Hj Hx"; trivial.
-    Unshelve.
-    all: try match goal with |- to_val _ = _ => simpl; by rewrite ?to_of_val end.
-    all: trivial.
+                    _ _ _ with "[$Hj $Hx]") as "[Hj Hx]"; eauto.
+    iMod (do_step_pure _ _ _ (CaseCtx _ _ :: K) with "[$Hj]") as "Hj"; eauto.
+    simpl.
+    iMod (do_step_pure with "[$Hj]") as "Hj"; eauto.
+    by iFrame "Hj Hx"; trivial.
   Qed.
 
+  Global Typeclasses Opaque CG_pop.
   Global Opaque CG_pop.
 
   Lemma CG_locked_pop_to_val st l :
@@ -250,17 +231,11 @@ Section CG_Stack.
     eapply with_lock_type; auto using CG_pop_type.
   Qed.
 
-  Lemma CG_locked_pop_closed (st l : expr) :
-    (∀ f, st.[f] = st) → (∀ f, l.[f] = l) →
-    ∀ f, (CG_locked_pop st l).[f] = CG_locked_pop st l.
-  Proof.
-    intros H1 H2 f. asimpl. unfold CG_locked_pop.
-    rewrite with_lock_closed; trivial. apply CG_pop_closed; trivial.
-  Qed.
-
   Lemma CG_locked_pop_subst (st l : expr) f :
-  (CG_locked_pop st l).[f] = CG_locked_pop st.[f] l.[f].
-  Proof. by rewrite with_lock_subst CG_pop_subst. Qed.
+    (CG_locked_pop st l).[f] = CG_locked_pop st.[f] l.[f].
+  Proof. by rewrite /CG_locked_pop; asimpl. Qed.
+
+  Hint Rewrite CG_locked_pop_subst : autosubst.
 
   Lemma steps_CG_locked_pop_suc E ρ j K st v w l :
     nclose specN ⊆ E →
@@ -269,12 +244,11 @@ Section CG_Stack.
       ⊢ |={E}=> j ⤇ fill K (InjR (of_val w)) ∗ st ↦ₛ v ∗ l ↦ₛ (#♭v false).
   Proof.
     iIntros (HNE) "[#Hspec [Hx [Hl Hj]]]". unfold CG_locked_pop.
-    iMod (steps_with_lock _ _ j K _ _ _ _ (InjRV w) UnitV _ _
-          with "[Hj Hx Hl]") as "Hj"; last done.
-    - iIntros (K') "[#Hspec Hxj]".
-      iApply steps_CG_pop_suc; first done. by iFrame.
-    - iFrame "Hspec Hj Hx"; trivial.
-      Unshelve. all: trivial.
+    iMod (steps_with_lock _ _ _ _ _ _ (st ↦ₛ FoldV (InjRV (PairV w v)))%I
+                          _ (InjRV w) UnitV
+            with "[$Hj $Hx $Hl]") as "Hj"; eauto.
+    iIntros (K') "[#Hspec Hxj]".
+    iApply steps_CG_pop_suc; eauto.
   Qed.
 
   Lemma steps_CG_locked_pop_fail E ρ j K st l :
@@ -284,14 +258,14 @@ Section CG_Stack.
       ⊢ |={E}=> j ⤇ fill K (InjL Unit) ∗ st ↦ₛ FoldV (InjLV UnitV) ∗ l ↦ₛ (#♭v false).
   Proof.
     iIntros (HNE) "[#Hspec [Hx [Hl Hj]]]". unfold CG_locked_pop.
-    iMod (steps_with_lock _ _ j K _ _ _ _ (InjLV UnitV) UnitV _ _
-          with "[Hj Hx Hl]") as "Hj"; last done.
-    - iIntros (K') "[#Hspec Hxj] /=".
-      iApply steps_CG_pop_fail; first done. by iFrame.
-    - iFrame "Hspec Hj Hx"; trivial.
-      Unshelve. all: trivial.
+    iMod (steps_with_lock _ _ _ _ _ _ (st ↦ₛ FoldV (InjLV UnitV))%I _
+                          (InjLV UnitV) UnitV
+          with "[$Hj $Hx $Hl]") as "Hj"; eauto.
+    iIntros (K') "[#Hspec Hxj] /=".
+      iApply steps_CG_pop_fail; eauto.
   Qed.
 
+  Global Typeclasses Opaque CG_locked_pop.
   Global Opaque CG_locked_pop.
 
   Lemma CG_snap_to_val st l : to_val (CG_snap st l) = Some (CG_snapV st l).
@@ -300,6 +274,7 @@ Section CG_Stack.
   Lemma CG_snap_of_val st l : of_val (CG_snapV st l) = CG_snap st l.
   Proof. trivial. Qed.
 
+  Global Typeclasses Opaque CG_snapV.
   Global Opaque CG_snapV.
 
   Lemma CG_snap_type st l Γ τ :
@@ -309,21 +284,14 @@ Section CG_Stack.
   Proof.
     intros H1 H2. repeat econstructor.
     eapply with_lock_type; trivial. do 2 constructor.
-    eapply (context_weakening [_; _]); eauto.
-  Qed.
-
-  Lemma CG_snap_closed (st l : expr) :
-    (∀ f, st.[f] = st) → (∀ f, l.[f] = l) →
-    ∀ f, (CG_snap st l).[f] = CG_snap st l.
-  Proof.
-    intros H1 H2 f. asimpl. unfold CG_snap.
-    rewrite with_lock_closed; trivial.
-    intros f'. by asimpl; rewrite ?H1.
+    eapply (context_weakening [_]); eauto.
   Qed.
 
   Lemma CG_snap_subst (st l : expr) f :
     (CG_snap st l).[f] = CG_snap st.[f] l.[f].
-  Proof. unfold CG_snap; rewrite ?with_lock_subst. by asimpl. Qed.
+  Proof. by unfold CG_snap; asimpl. Qed.
+
+  Hint Rewrite CG_snap_subst : autosubst.
 
   Lemma steps_CG_snap E ρ j K st v l :
     nclose specN ⊆ E →
@@ -332,20 +300,16 @@ Section CG_Stack.
       ⊢ |={E}=> j ⤇ (fill K (of_val v)) ∗ st ↦ₛ v ∗ l ↦ₛ (#♭v false).
   Proof.
     iIntros (HNE) "[#Hspec [Hx [Hl Hj]]]". unfold CG_snap.
-    iMod (steps_with_lock _ _ j K _ _ (st ↦ₛ v)%I _ v UnitV _ _
-          with "[Hj Hx Hl]") as "Hj"; last done; [|iFrame; iFrame "#"].
+    iMod (steps_with_lock _ _ _ _ _ _ (st ↦ₛ v)%I _ v UnitV
+          with "[$Hj $Hx $Hl]") as "Hj"; eauto.
     iIntros (K') "[#Hspec [Hx Hj]]".
-    iMod (step_rec _ _ j K' _ _ _ _ with "[Hj]") as "Hj"; eauto.
+    iMod (do_step_pure with "[$Hj]") as "Hj"; eauto.
     iAsimpl.
-    iMod (step_load _ _ j K' _ _ _ _
-          with "[Hj Hx]") as "[Hj Hx]"; eauto.
-    - iFrame "#"; iFrame.
-    - iModIntro. by iFrame "Hj Hx".
-      Unshelve.
-      all: try match goal with |- to_val _ = _ => simpl; by rewrite ?to_of_val end.
-      all: trivial.
+    iMod (step_load with "[$Hj $Hx]") as "[Hj Hx]"; eauto.
+    by iFrame.
   Qed.
 
+  Global Typeclasses Opaque CG_snap.
   Global Opaque CG_snap.
 
   (* Coarse-grained iter *)
@@ -354,8 +318,9 @@ Section CG_Stack.
     Rec (Case (Unfold (Var 1))
               Unit
               (
-                App (Rec (App (Var 3) (Snd (Var 2))))
-                    (App f.[ren (+3)] (Fst (Var 0)))
+                Seq
+                  (App f.[ren (+3)] (Fst (Var 0)))
+                  (App (Var 1) (Snd (Var 0)))
               )
         ).
   Proof. trivial. Qed.
@@ -364,15 +329,14 @@ Section CG_Stack.
     typed Γ f (TArrow τ TUnit) →
     typed Γ (CG_iter f) (TArrow (CG_StackType τ) TUnit).
   Proof.
-    intros H1.
-    econstructor.
-    eapply (Case_typed _ _ _ _ TUnit);
-      [| repeat constructor
-       | repeat econstructor; eapply (context_weakening [_; _; _]); eauto].
+    intros ?. econstructor.
+    eapply (Case_typed _ _ _ _ TUnit); eauto using typed.
     replace (TSum TUnit (TProd τ (CG_StackType τ))) with
     ((TSum TUnit (TProd τ.[ren (+1)] (TVar 0))).[(CG_StackType τ)/])
       by (by asimpl).
     repeat econstructor.
+    repeat econstructor; simpl; eauto using typed.
+    eapply (context_weakening [_; _; _]); eauto.
   Qed.
 
   Lemma CG_iter_to_val f : to_val (CG_iter f) = Some (CG_iterV f).
@@ -381,14 +345,13 @@ Section CG_Stack.
   Lemma CG_iter_of_val f : of_val (CG_iterV f) = CG_iter f.
   Proof. trivial. Qed.
 
+  Global Typeclasses Opaque CG_iterV.
   Global Opaque CG_iterV.
 
-  Lemma CG_iter_closed (f : expr) :
-    (∀ g, f.[g] = f) → ∀ g, (CG_iter f).[g] = CG_iter f.
-  Proof. intros Hf g. unfold CG_iter. asimpl. rewrite ?Hf; trivial. Qed.
-
   Lemma CG_iter_subst (f : expr) g : (CG_iter f).[g] = CG_iter f.[g].
-  Proof. unfold CG_iter; asimpl; trivial. Qed.
+  Proof. by unfold CG_iter; asimpl. Qed.
+
+  Hint Rewrite CG_iter_subst : autosubst.
 
   Lemma steps_CG_iter E ρ j K f v w :
     nclose specN ⊆ E →
@@ -397,27 +360,19 @@ Section CG_Stack.
                                (Fold (InjR (Pair (of_val w) (of_val v)))))
       ⊢ |={E}=>
     j ⤇ fill K
-          (App
-             (Rec
-                (App ((CG_iter (of_val f)).[ren (+2)])
-                     (Snd (Pair ((of_val w).[ren (+2)]) (of_val v).[ren (+2)]))))
-             (App (of_val f) (of_val w))).
+          (Seq (App (of_val f) (of_val w))
+               (App (CG_iter (of_val f)) (Snd (Pair (of_val w) (of_val v))))).
   Proof.
     iIntros (HNE) "[#Hspec Hj]". unfold CG_iter.
-    iMod (step_rec _ _ j K _ _ _ _ with "[Hj]") as "Hj"; eauto.
-    rewrite -CG_iter_folding. Opaque CG_iter. iAsimpl.
-    iMod (step_Fold _ _ j (CaseCtx _ _ :: K)
-                    _ _ _ with "[Hj]") as "Hj"; eauto.
+    iMod (do_step_pure with "[$Hj]") as "Hj"; eauto.
     iAsimpl.
-    iMod (step_case_inr _ _ j K _ _ _ _ _ with "[Hj]") as "Hj"; eauto.
+    iMod (do_step_pure _ _ _ (CaseCtx _ _ :: K) with "[$Hj]") as "Hj"; eauto.
     iAsimpl.
-    iMod (step_fst _ _ j (AppRCtx f :: AppRCtx (RecV _) :: K) _ _ _ _
-                   _ _ with "[Hj]") as "Hj"; eauto.
-    Unshelve.
-    all: try match goal with |- to_val _ = _ => simpl; by rewrite ?to_of_val end.
+    iMod (do_step_pure with "[$Hj]") as "Hj"; eauto.
+    iAsimpl.
+    iMod (do_step_pure _ _ _ (AppRCtx f :: SeqCtx _ :: K) with "[$Hj]")
+      as "Hj"; eauto.
   Qed.
-
-  Transparent CG_iter.
 
   Lemma steps_CG_iter_end E ρ j K f :
     nclose specN ⊆ E →
@@ -425,16 +380,13 @@ Section CG_Stack.
       ⊢ |={E}=> j ⤇ fill K Unit.
   Proof.
     iIntros (HNE) "[#Hspec Hj]". unfold CG_iter.
-    iMod (step_rec _ _ j K _ _ _ _ with "[Hj]") as "Hj"; eauto.
-    rewrite -CG_iter_folding. Opaque CG_iter. iAsimpl.
-    iMod (step_Fold _ _ j (CaseCtx _ _ :: K)
-                    _ _ _ with "[Hj]") as "Hj"; eauto.
+    iMod (do_step_pure with "[$Hj]") as "Hj"; eauto.
+    iMod (do_step_pure _ _ _ (CaseCtx _ _ :: K) with "[$Hj]") as "Hj"; eauto.
     iAsimpl.
-    iMod (step_case_inl _ _ j K _ _ _ _ _ with "[Hj]") as "Hj"; eauto.
-    Unshelve.
-    all: try match goal with |- to_val _ = _ => simpl; by rewrite ?to_of_val end.
+    iMod (do_step_pure with "[$Hj]") as "Hj"; eauto.
   Qed.
 
+  Global Typeclasses Opaque CG_iter.
   Global Opaque CG_iter.
 
   Lemma CG_snap_iter_type st l Γ τ :
@@ -444,23 +396,14 @@ Section CG_Stack.
   Proof.
     intros H1 H2; repeat econstructor.
     - eapply CG_iter_type; by constructor.
-    - eapply CG_snap_type; by eapply (context_weakening [_;_]).
-  Qed.
-
-  Lemma CG_snap_iter_closed (st l : expr) :
-    (∀ f, st.[f] = st) → (∀ f, l.[f] = l) →
-    ∀ f, (CG_snap_iter st l).[f] = CG_snap_iter st l.
-  Proof.
-    intros H1 H2 f. unfold CG_snap_iter. asimpl. rewrite H1 H2.
-    rewrite CG_snap_closed; auto.
+    - eapply CG_snap_type; by eapply (context_weakening [_]).
   Qed.
 
   Lemma CG_snap_iter_subst (st l : expr) g :
     (CG_snap_iter st l).[g] = CG_snap_iter st.[g] l.[g].
-  Proof.
-    unfold CG_snap_iter; asimpl.
-    rewrite CG_snap_subst CG_iter_subst. by asimpl.
-  Qed.
+  Proof. by unfold CG_snap_iter; asimpl. Qed.
+
+  Hint Rewrite CG_snap_iter_subst : autosubst.
 
   Lemma CG_stack_body_type st l Γ τ :
     typed Γ st (Tref (CG_StackType τ)) →
@@ -476,17 +419,15 @@ Section CG_Stack.
                           CG_locked_pop_type, CG_snap_iter_type).
   Qed.
 
-  Opaque CG_snap_iter.
 
-  Lemma CG_stack_body_closed (st l : expr) :
-    (∀ f, st.[f] = st) → (∀ f, l.[f] = l) →
-    ∀ f, (CG_stack_body st l).[f] = CG_stack_body st l.
-  Proof.
-    intros H1 H2 f. unfold CG_stack_body. asimpl.
-    rewrite CG_locked_push_closed; trivial.
-    rewrite CG_locked_pop_closed; trivial.
-    by rewrite CG_snap_iter_closed.
-  Qed.
+  Global Typeclasses Opaque CG_snap_iter.
+  Global Opaque CG_snap_iter.
+
+  Lemma CG_stack_body_subst (st l : expr) f :
+    (CG_stack_body st l).[f] = CG_stack_body st.[f] l.[f].
+  Proof. by unfold CG_stack_body; asimpl. Qed.
+
+  Hint Rewrite CG_stack_body_subst : autosubst.
 
   Lemma CG_stack_type Γ :
     typed Γ CG_stack
@@ -499,18 +440,24 @@ Section CG_Stack.
                 (TArrow (TArrow (TVar 0) TUnit) TUnit)
           )).
   Proof.
-    repeat econstructor.
-    - eapply CG_locked_push_type; constructor; simpl; eauto.
-    - eapply CG_locked_pop_type; constructor; simpl; eauto.
-    - eapply CG_snap_iter_type; constructor; by simpl.
-    - asimpl. repeat constructor.
-    - eapply newlock_type.
+    repeat econstructor;
+      eauto 10 using newlock_type, CG_locked_push_type, CG_locked_pop_type,
+      CG_snap_iter_type, typed.
+    asimpl; repeat constructor.
   Qed.
 
   Lemma CG_stack_closed f : CG_stack.[f] = CG_stack.
-  Proof.
-    unfold CG_stack.
-    asimpl; rewrite ?CG_locked_push_subst ?CG_locked_pop_subst.
-    asimpl. rewrite ?CG_snap_iter_subst. by asimpl.
-  Qed.
+  Proof. by unfold CG_stack; asimpl. Qed.
+
 End CG_Stack.
+
+Global Hint Rewrite CG_push_subst : autosubst.
+Global Hint Rewrite CG_locked_push_subst : autosubst.
+Global Hint Rewrite CG_locked_pop_subst : autosubst.
+Global Hint Rewrite CG_pop_subst : autosubst.
+Global Hint Rewrite CG_locked_pop_subst : autosubst.
+Global Hint Rewrite CG_snap_subst : autosubst.
+Global Hint Rewrite CG_iter_subst : autosubst.
+Global Hint Rewrite CG_snap_iter_subst : autosubst.
+Global Hint Rewrite CG_stack_body_subst : autosubst.
+Global Hint Rewrite CG_stack_closed : autosubst.
