theories/logrel/F_mu_ref_conc/examples/stack/FG_stack.v
@@ -1,4 +1,4 @@
-From iris_examples.logrel.F_mu_ref_conc Require Import  typing.
+From iris_examples.logrel.F_mu_ref_conc Require Import typing.
 
 Definition FG_StackType τ :=
   TRec (Tref (TSum TUnit (TProd τ.[ren (+1)] (TVar 0)))).
@@ -7,103 +7,99 @@ Definition FG_Stack_Ref_Type τ :=
   Tref (TSum TUnit (TProd τ (FG_StackType τ))).
 
 Definition FG_push (st : expr) : expr :=
-  Rec (App (Rec
-              (* try push *)
-              (If (CAS (st.[ren (+4)]) (Var 1)
-                       (Alloc (InjR (Pair (Var 3) (Fold (Var 1)))))
-                  )
-                  Unit (* push succeeds we return unit *)
-                  (App (Var 2) (Var 3)) (* push fails, we try again *)
-              )
+  Rec
+    (LetIn
+       (Load st.[ren (+2)])
+       (* try push *)
+       (If (CAS (st.[ren (+3)]) (Var 0)
+                (Alloc (InjR (Pair (Var 2) (Fold (Var 0)))))
            )
-           (Load st.[ren (+2)]) (* read the stack pointer *)
-      ).
+           Unit (* push succeeds we return unit *)
+           (App (Var 1) (Var 2)) (* push fails, we try again *)
+       )
+    ).
+
 Definition FG_pushV (st : expr) : val :=
-  RecV (App (Rec
-              (* try push *)
-              (If (CAS (st.[ren (+4)]) (Var 1)
-                       (Alloc (InjR (Pair (Var 3) (Fold (Var 1)))))
-                  )
-                  Unit (* push succeeds we return unit *)
-                  (App (Var 2) (Var 3)) (* push fails, we try again *)
-              )
+  RecV
+    (LetIn
+       (Load st.[ren (+2)])
+       (* try push *)
+       (If (CAS (st.[ren (+3)]) (Var 0)
+                (Alloc (InjR (Pair (Var 2) (Fold (Var 0)))))
            )
-           (Load st.[ren (+2)]) (* read the stack pointer *)
-       ).
+           Unit (* push succeeds we return unit *)
+           (App (Var 1) (Var 2)) (* push fails, we try again *)
+       )
+    ).
 
 Definition FG_pop (st : expr) : expr :=
-  Rec (App (Rec
-              (App
-                 (Rec
-                    (
-                      Case (Var 1)
-                           (InjL Unit)
-                           ( (* try popping *)
-                             If
-                               (CAS
-                                  (st.[ren (+7)])
-                                  (Var 4)
-                                  (Unfold (Snd (Var 0)))
-                               )
-                               (InjR (Fst (Var 0))) (* pop succeeds *)
-                               (App (Var 5) (Var 6)) (* pop fails, we retry*)
-                           )
-                     )
+  Rec
+    (LetIn
+       (Load st.[ren (+ 2)])
+       (LetIn
+          (Load (Var 0))
+          (Case
+             (Var 0)
+             (InjL Unit)
+             ( (* try popping *)
+               If
+                 (CAS
+                    (st.[ren (+5)])
+                    (Var 2)
+                    (Unfold (Snd (Var 0)))
                  )
-                 (
-                   (Load (Var 1))
-                 )
-              )
-           )
-           (Load st.[ren (+ 2)])
-      ).
-Definition FG_popV (st : expr) : val :=
-  RecV
-    (App
-       (Rec
-          ( App
-              (Rec
-                 (
-                   Case (Var 1)
-                        (InjL Unit)
-                        ( (* try popping *)
-                          If
-                            (CAS
-                               (st.[ren (+7)])
-                               (Var 4)
-                               (Unfold (Snd (Var 0)))
-                            )
-                            (InjR (Fst (Var 0))) (* pop succeeds *)
-                            (App (Var 5) (Var 6)) (* pop fails, we retry*)
-                        )
-                 )
-              )
-              (
-                (Load (Var 1))
-              )
+                 (InjR (Fst (Var 0))) (* pop succeeds *)
+                 (App (Var 3) (Var 4)) (* pop fails, we retry*)
+             )
           )
        )
+    ).
+
+Definition FG_popV (st : expr) : val :=
+  RecV
+    (LetIn
        (Load st.[ren (+ 2)])
+       (LetIn
+          (Load (Var 0))
+          (Case
+             (Var 0)
+             (InjL Unit)
+             ( (* try popping *)
+               If
+                 (CAS
+                    (st.[ren (+5)])
+                    (Var 2)
+                    (Unfold (Snd (Var 0)))
+                 )
+                 (InjR (Fst (Var 0))) (* pop succeeds *)
+                 (App (Var 3) (Var 4)) (* pop fails, we retry*)
+             )
+          )
+       )
     ).
 
 Definition FG_iter (f : expr) : expr :=
   Rec
     (Case (Load (Unfold (Var 1)))
           Unit
-          (App (Rec (App (Var 3) (Snd (Var 2)))) (* recursive_call *)
-               (App f.[ren (+3)] (Fst (Var 0)))
+          (Seq
+             (App f.[ren (+3)] (Fst (Var 0)))
+             (App (Var 1) (Snd (Var 0))) (* recursive_call *)
           )
     ).
+
 Definition FG_iterV (f : expr) : val :=
   RecV
     (Case (Load (Unfold (Var 1)))
           Unit
-          (App (Rec (App (Var 3) (Snd (Var 2)))) (* recursive_call *)
-               (App f.[ren (+3)] (Fst (Var 0)))
+          (Seq
+             (App f.[ren (+3)] (Fst (Var 0)))
+             (App (Var 1) (Snd (Var 0))) (* recursive_call *)
           )
     ).
+
 Definition FG_read_iter (st : expr) : expr :=
-  Rec (App (FG_iter (Var 1)) (Fold (Load st.[ren (+2)]))).
+  Lam (App (FG_iter (Var 0)) (Fold (Load st.[ren (+1)]))).
 
 Definition FG_stack_body (st : expr) : expr :=
   Pair (Pair (FG_push st) (FG_pop st)) (FG_read_iter st).
@@ -116,34 +112,19 @@ Section FG_stack.
   (* Fine-grained push *)
   Lemma FG_push_folding (st : expr) :
     FG_push st =
-    Rec (App (Rec
-                (* try push *)
-                (If (CAS (st.[ren (+4)]) (Var 1)
-                         (Alloc (InjR (Pair (Var 3) (Fold (Var 1)))))
-                    )
-                    Unit (* push succeeds we return unit *)
-                    (App (Var 2) (Var 3)) (* push fails, we try again *)
-                )
-             )
-             (Load st.[ren (+2)]) (* read the stack pointer *)
-        ).
+    Rec
+    (LetIn
+       (Load st.[ren (+2)])
+       (* try push *)
+       (If (CAS (st.[ren (+3)]) (Var 0)
+                (Alloc (InjR (Pair (Var 2) (Fold (Var 0)))))
+           )
+           Unit (* push succeeds we return unit *)
+           (App (Var 1) (Var 2)) (* push fails, we try again *)
+       )
+    ).
   Proof. trivial. Qed.
 
-  Section FG_push_type.
-    Lemma FG_push_type st Γ τ :
-      typed Γ st (Tref (FG_Stack_Ref_Type τ)) →
-      typed Γ (FG_push st) (TArrow τ TUnit).
-    Proof.
-      intros HTst.
-      repeat match goal with
-               |- typed _ _ _ => econstructor; eauto
-             end; repeat econstructor; eauto.
-      - eapply (context_weakening [_; _; _; _]); eauto.
-      - by asimpl.
-      -  eapply (context_weakening [_; _]); eauto.
-    Qed.
-
-  End FG_push_type.
 
   Lemma FG_push_to_val st : to_val (FG_push st) = Some (FG_pushV st).
   Proof. trivial. Qed.
@@ -151,83 +132,95 @@ Section FG_stack.
   Lemma FG_push_of_val st : of_val (FG_pushV st) = FG_push st.
   Proof. trivial. Qed.
 
+  Global Typeclasses Opaque FG_pushV.
   Global Opaque FG_pushV.
 
-  Lemma FG_push_closed (st : expr) :
-    (∀ f, st.[f] = st) → ∀ f, (FG_push st).[f] = FG_push st.
-  Proof. intros H f. asimpl. unfold FG_push. rewrite ?H; trivial. Qed.
+  Lemma FG_push_type st Γ τ :
+    typed Γ st (Tref (FG_Stack_Ref_Type τ)) →
+    typed Γ (FG_push st) (TArrow τ TUnit).
+  Proof.
+    intros ?.
+    do 2 econstructor.
+    { econstructor; eapply (context_weakening [_; _]); eauto. }
+    econstructor; eauto using typed.
+    econstructor; eauto using typed; repeat econstructor.
+    - eapply (context_weakening [_; _; _]); eauto.
+    - by asimpl.
+  Qed.
 
-  Lemma FG_push_subst (st : expr) f : (FG_push st).[f] = FG_push st.[f].
-  Proof. unfold FG_push. by asimpl. Qed.
+  Lemma FG_push_subst (st : expr) f :
+    (FG_push st).[f] = FG_push st.[f].
+  Proof. by rewrite /FG_push; asimpl. Qed.
 
+  Hint Rewrite FG_push_subst : autosubst.
+
+  Global Typeclasses Opaque FG_push.
   Global Opaque FG_push.
 
   (* Fine-grained push *)
   Lemma FG_pop_folding (st : expr) :
     FG_pop st =
-    Rec (App (Rec
-                ( App
-                    (Rec
-                       (
-                         Case (Var 1)
-                              (InjL Unit)
-                              ( (* try popping *)
-                                If
-                                  (CAS
-                                     (st.[ren (+7)])
-                                     (Var 4)
-                                     (Unfold (Snd (Var 0)))
-                                  )
-                                  (InjR (Fst (Var 0))) (* pop succeeds *)
-                                  (App (Var 5) (Var 6)) (* pop fails, we retry*)
-                              )
-                       )
-                    )
-                    (
-                      (Load (Var 1))
-                    )
-                )
-             )
-             (Load st.[ren (+ 2)])
-        ).
+    Rec
+      (LetIn
+         (Load st.[ren (+ 2)])
+         (LetIn
+            (Load (Var 0))
+            (Case
+               (Var 0)
+               (InjL Unit)
+               ( (* try popping *)
+                 If
+                   (CAS
+                      (st.[ren (+5)])
+                      (Var 2)
+                    (Unfold (Snd (Var 0)))
+                   )
+                   (InjR (Fst (Var 0))) (* pop succeeds *)
+                   (App (Var 3) (Var 4)) (* pop fails, we retry*)
+               )
+            )
+         )
+      ).
   Proof. trivial. Qed.
-
-  Section FG_pop_type.
-
-    Lemma FG_pop_type st Γ τ :
-      typed Γ st (Tref (FG_Stack_Ref_Type τ)) →
-      typed Γ (FG_pop st) (TArrow TUnit (TSum TUnit τ)).
-    Proof.
-      replace (FG_Stack_Ref_Type τ) with
-          (Tref (TSum TUnit (TProd τ.[ren (+1)] (TVar 0)))).[FG_StackType τ/];
-        last first.
-      { by asimpl. }
-      intros HTst.
-      repeat match goal with
-               |- typed _ _ _ => econstructor; eauto
-             end; repeat econstructor; eauto; last first.
-      - eapply (context_weakening [_; _]); eauto.
-      - by asimpl.
-      - eapply (context_weakening [_; _; _; _; _; _; _]); eauto.
-      - econstructor.
-    Qed.
-  End FG_pop_type.
 
   Lemma FG_pop_to_val st : to_val (FG_pop st) = Some (FG_popV st).
   Proof. trivial. Qed.
-
   Lemma FG_pop_of_val st : of_val (FG_popV st) = FG_pop st.
   Proof. trivial. Qed.
 
+  Global Typeclasses Opaque FG_popV.
   Global Opaque FG_popV.
 
-  Lemma FG_pop_closed (st : expr) :
-    (∀ f, st.[f] = st) → ∀ f, (FG_pop st).[f] = FG_pop st.
-  Proof. intros H f. asimpl. unfold FG_pop. rewrite ?H; trivial. Qed.
+  Lemma FG_pop_type st Γ τ :
+    typed Γ st (Tref (FG_Stack_Ref_Type τ)) →
+    typed Γ (FG_pop st) (TArrow TUnit (TSum TUnit τ)).
+  Proof.
+    replace (FG_Stack_Ref_Type τ) with
+        (Tref (TSum TUnit (TProd τ.[ren (+1)] (TVar 0)))).[FG_StackType τ/];
+      last first.
+    { by asimpl. }
+    intros ?.
+    do 2 econstructor.
+    { econstructor. eapply (context_weakening [_; _]); eauto. }
+    econstructor.
+    { repeat econstructor. }
+    econstructor.
+    { repeat econstructor. }
+    { repeat econstructor. }
+    econstructor.
+    - econstructor;
+        [|eapply (context_weakening [_; _; _; _; _]); eauto| |];
+        repeat econstructor.
+    - by repeat econstructor; asimpl.
+    - repeat econstructor.
+  Qed.
 
   Lemma FG_pop_subst (st : expr) f : (FG_pop st).[f] = FG_pop st.[f].
   Proof. unfold FG_pop. by asimpl. Qed.
 
+  Hint Rewrite FG_pop_subst : autosubst.
+
+  Global Typeclasses Opaque FG_pop.
   Global Opaque FG_pop.
 
   (* Fine-grained iter *)
@@ -236,8 +229,9 @@ Section FG_stack.
     Rec
       (Case (Load (Unfold (Var 1)))
             Unit
-            (App (Rec (App (Var 3) (Snd (Var 2)))) (* recursive_call *)
-                 (App f.[ren (+3)] (Fst (Var 0)))
+            (Seq
+               (App f.[ren (+3)] (Fst (Var 0)))
+               (App (Var 1) (Snd (Var 0))) (* recursive_call *)
             )
       ).
   Proof. trivial. Qed.
@@ -265,14 +259,12 @@ Section FG_stack.
   Proof. trivial. Qed.
 
   Global Opaque FG_popV.
-
-  Lemma FG_iter_closed (f : expr) :
-    (∀ g, f.[g] = f) → ∀ g, (FG_iter f).[g] = FG_iter f.
-  Proof. intros H g. asimpl. unfold FG_iter. rewrite ?H; trivial. Qed.
-
   Lemma FG_iter_subst (f : expr) g : (FG_iter f).[g] = FG_iter f.[g].
   Proof. unfold FG_iter. by asimpl. Qed.
 
+  Hint Rewrite FG_iter_subst : autosubst.
+
+  Global Typeclasses Opaque FG_iter.
   Global Opaque FG_iter.
 
   Lemma FG_read_iter_type st Γ τ :
@@ -282,77 +274,64 @@ Section FG_stack.
   Proof.
     intros H1; repeat econstructor.
     - eapply FG_iter_type; by constructor.
-    - by eapply (context_weakening [_;_]); asimpl.
-  Qed.
-
-  Transparent FG_iter.
-
-  Lemma FG_read_iter_closed (st : expr) :
-    (∀ f, st.[f] = st) →
-    ∀ f, (FG_read_iter st).[f] = FG_read_iter st.
-  Proof.
-    intros H1 f. unfold FG_read_iter, FG_iter. asimpl.
-    by rewrite ?H1.
+    - by eapply (context_weakening [_]); asimpl.
   Qed.
 
   Lemma FG_read_iter_subst (st : expr) g :
     (FG_read_iter st).[g] = FG_read_iter st.[g].
   Proof. by unfold FG_read_iter; asimpl. Qed.
 
-  Global Opaque FG_iter.
+  Hint Rewrite FG_read_iter_subst : autosubst.
 
-  Section FG_stack_body_type.
+  Global Typeclasses Opaque FG_read_iter.
+  Global Opaque FG_read_iter.
 
-    Lemma FG_stack_body_type st Γ τ :
-      typed Γ st (Tref (FG_Stack_Ref_Type τ)) →
-      typed Γ (FG_stack_body st)
-            (TProd
-               (TProd (TArrow τ TUnit) (TArrow TUnit (TSum TUnit τ)))
-               (TArrow (TArrow τ TUnit) TUnit)
-            ).
-    Proof.
-      intros H1.
-      repeat (econstructor; eauto using FG_push_type,
-                            FG_pop_type, FG_read_iter_type).
-    Qed.
-  End FG_stack_body_type.
+  Lemma FG_stack_body_type st Γ τ :
+    typed Γ st (Tref (FG_Stack_Ref_Type τ)) →
+    typed Γ (FG_stack_body st)
+          (TProd
+             (TProd (TArrow τ TUnit) (TArrow TUnit (TSum TUnit τ)))
+             (TArrow (TArrow τ TUnit) TUnit)
+          ).
+  Proof.
+    intros H1.
+    repeat (econstructor; eauto using FG_push_type,
+                          FG_pop_type, FG_read_iter_type).
+  Qed.
 
   Opaque FG_read_iter.
 
-  Lemma FG_stack_body_closed (st : expr) :
-    (∀ f, st.[f] = st) →
-    ∀ f, (FG_stack_body st).[f] = FG_stack_body st.
+  Lemma FG_stack_body_subst (st : expr) f :
+    (FG_stack_body st).[f] = FG_stack_body st.[f].
+  Proof. by unfold FG_stack_body; asimpl. Qed.
+
+  Hint Rewrite FG_stack_body_subst : autosubst.
+
+  Lemma FG_stack_type Γ :
+    typed Γ FG_stack
+          (TForall
+             (TProd
+                (TProd
+                   (TArrow (TVar 0) TUnit)
+                   (TArrow TUnit (TSum TUnit (TVar 0)))
+                )
+                (TArrow (TArrow (TVar 0) TUnit) TUnit)
+          )).
   Proof.
-    intros H1 f. unfold FG_stack_body. asimpl.
-    rewrite FG_push_closed; trivial.
-    rewrite FG_pop_closed; trivial.
-    by rewrite FG_read_iter_closed.
+    repeat econstructor.
+    - eapply FG_push_type; try constructor; simpl; eauto.
+    - eapply FG_pop_type; try constructor; simpl; eauto.
+    - eapply FG_read_iter_type; constructor; by simpl.
   Qed.
-
-  Section FG_stack_type.
-
-    Lemma FG_stack_type Γ :
-      typed Γ FG_stack
-            (TForall
-               (TProd
-                  (TProd
-                     (TArrow (TVar 0) TUnit)
-                     (TArrow TUnit (TSum TUnit (TVar 0)))
-                  )
-                  (TArrow (TArrow (TVar 0) TUnit) TUnit)
-            )).
-    Proof.
-      repeat econstructor.
-      - eapply FG_push_type; try constructor; simpl; eauto.
-      - eapply FG_pop_type; try constructor; simpl; eauto.
-      - eapply FG_read_iter_type; constructor; by simpl.
-    Qed.
-  End FG_stack_type.
 
   Lemma FG_stack_closed f : FG_stack.[f] = FG_stack.
-  Proof.
-    unfold FG_stack.
-    asimpl; rewrite ?FG_push_subst ?FG_pop_subst.
-    asimpl. rewrite ?FG_read_iter_subst. by asimpl.
-  Qed.
+  Proof. by unfold FG_stack; asimpl. Qed.
+
 End FG_stack.
+
+Global Hint Rewrite FG_push_subst : autosubst.
+Global Hint Rewrite FG_pop_subst : autosubst.
+Global Hint Rewrite FG_iter_subst : autosubst.
+Global Hint Rewrite FG_read_iter_subst : autosubst.
+Global Hint Rewrite FG_stack_body_subst : autosubst.
+Global Hint Rewrite FG_stack_closed : autosubst.
